Simple_Clause_Learning/Alternative_Backtracking_Function.thy
@@ -1,0 +1,138 @@
+theory Alternative_Backtracking_Function
+  imports Simple_Clause_Learning
+begin
+
+primrec bt where
+  "bt [] n = ([], 0)" |
+  "bt (Ln # \<Gamma>) n =
+    (let (\<Gamma>', n') = bt \<Gamma> n in
+     if \<Gamma> = \<Gamma>' then
+       (\<Gamma>', n')
+     
+     if is_decision_lit Ln then
+       if n' < n then
+         (Ln # \<Gamma>', Suc n')
+       else
+         (\<Gamma>', n')
+     else if n' \<le> n then
+       (Ln # \<Gamma>', n')
+     else
+       (\<Gamma>', n'))"
+
+value [simp] "bt [(w, Some ({#}, w, Var)), (z, None), (y, Some ({#}, y, Var)), (x, None)] 0"
+
+lemma bt_level_inv: "bt \<Gamma> level = (\<Gamma>', level') \<Longrightarrow> trail_level \<Gamma>' = level'"
+proof (induction \<Gamma> arbitrary: \<Gamma>' level')
+  case Nil
+  then show ?case by simp
+next
+  case (Cons Ln \<Gamma>)
+  obtain \<Gamma>'' level'' where "bt \<Gamma> level = (\<Gamma>'', level'')"
+    by fastforce
+  with Cons.prems show ?case
+    apply simp
+    by (smt (verit, best) Cons.IH Pair_inject id_apply trail_level.simps(2))
+qed
+
+abbreviation trail_backtrack where
+  "trail_backtrack \<Gamma> level \<equiv> fst (bt \<Gamma> level)"
+
+lemma trail_level_trail_backtrack_le[simp]: "trail_level (trail_backtrack \<Gamma> level) \<le> level"
+proof (induction \<Gamma>)
+  case Nil
+  show ?case
+    by simp
+next
+  case (Cons Ln \<Gamma>)
+  thus ?case
+    by (smt (verit) Pair_inject Suc_le_eq bt.simps(2) bt_level_inv prod.case_eq_if prod.collapse)
+qed
+
+lemma trail_backtrack_ident: "trail_level \<Gamma> < level \<Longrightarrow> trail_backtrack \<Gamma> level = \<Gamma>"
+proof (induction \<Gamma>)
+  case Nil
+  show ?case by simp
+next
+  case (Cons Ln \<Gamma>)
+  then show ?case
+    apply simp
+    by (smt (verit, del_insts) Pair_inject Suc_le_lessD bt_level_inv case_prod_conv id_apply
+        le_eq_less_or_eq prod.collapse)
+qed
+
+lemma trail_backtrack_identD: "trail_backtrack \<Gamma> level = \<Gamma> \<Longrightarrow> trail_level \<Gamma> \<le> level"
+  apply (induction \<Gamma>)
+   apply simp
+  apply simp
+  apply auto
+   apply (smt (verit, ccfv_SIG) bt_level_inv case_prod_conv fst_conv less_Suc_eq_le not_less_eq
+      prod.collapse trail_level.simps(2) trail_level_trail_backtrack_le)
+  by (smt (verit, del_insts) bt_level_inv fst_conv list.inject prod.collapse split_beta
+      trail_level_trail_backtrack_le)
+
+lemma bt_level_inv2: "bt \<Gamma> level = (\<Gamma>', level') \<Longrightarrow> if level < level' then \<Gamma> = \<Gamma>' else suffix \<Gamma>' \<Gamma>"
+proof (induction \<Gamma> arbitrary: \<Gamma>' level')
+  case Nil
+  thus ?case by simp
+next
+  case (Cons Ln \<Gamma>)
+  obtain \<Gamma>'' level'' where "bt \<Gamma> level = (\<Gamma>'', level'')"
+    by fastforce
+
+  hence "level'' \<le> level"
+    using trail_level_trail_backtrack_le[of \<Gamma> level] bt_level_inv[of \<Gamma> level] by auto
+
+  with Cons.prems show ?case
+    apply (simp add: \<open>bt \<Gamma> level = (\<Gamma>'', level'')\<close>)
+    apply (cases "is_decision_lit Ln"; simp)
+    using Cons.IH[OF \<open>bt \<Gamma> level = (\<Gamma>'', level'')\<close>]
+     apply (cases "level = level''"; simp)
+      apply (simp add: suffix_Cons)
+    unfolding suffix_def
+     defer
+    apply simp
+
+    
+    using trail_level_trail_backtrack_le[of \<Gamma> level]
+    using bt_level_inv[OF \<open>bt \<Gamma> level = (\<Gamma>'', level'')\<close>]
+    apply simp
+    apply (cases "is_decision_lit Ln"; simp)
+    subgoal apply (cases "level = level''"; simp) sorry
+    subgoal
+      apply simp
+    
+    
+    sorry
+qed
+
+lemma trail_backtrack_suffix: "suffix (trail_backtrack \<Gamma> level) \<Gamma>"
+proof (induction \<Gamma>)
+  case Nil
+  show ?case by simp
+next
+  case (Cons Ln \<Gamma>)
+  obtain \<Gamma>'' level'' where "bt \<Gamma> level = (\<Gamma>'', level'')"
+    by fastforce
+  with Cons show ?case
+    apply (cases "is_decision_lit Ln")
+     apply (simp_all add: suffix_ConsI)
+    unfolding suffix_def
+qed
+  oops
+
+lemma (in scl)
+  assumes sound_\<Gamma>: "sound_trail N U \<Gamma>"
+  shows "level < trail_level_lit \<Gamma> L \<Longrightarrow> \<not> trail_defined_lit (fst (bt \<Gamma> level)) L"
+  using sound_\<Gamma>
+proof (induction \<Gamma> rule: sound_trail.induct)
+  case Nil
+  then show ?case by simp
+next
+  case (Cons \<Gamma> K u)
+  obtain \<Gamma>' m where "bt \<Gamma> level = (\<Gamma>', m)" by force
+  with Cons.hyps(1) Cons.prems show ?case
+    apply simp
+    apply (rule conjI)
+    oops
+
+end
